BiDir Typing

Rocq/src/Expr.v
@@ -1,7 +1,9 @@
 From Stdlib Require Import Lists.List.
-From Stdlib Require Import Strings.String.
 From Verilog Require Import ident_to_string.
+From Verilog Require Import Utils.
+
 Import ListNotations.
+Import Utils.
 
 Set Implicit Arguments.
 
@@ -10,7 +12,7 @@ Module Expr.
   Unset Elimination Schemes.
 
   Inductive Expr : Type :=
-  | EOperand (op: string)
+  | EAtom (size: nat)
   | EBinOp (lhs rhs: Expr)
   | EUnOp (arg: Expr)
   | ECast (arg: Expr)
@@ -18,22 +20,22 @@ Module Expr.
   | ELogic (lhs rhs: Expr)
   | EReduction (arg: Expr)
   | EShift (lhs rhs: Expr)
-  | EAssign (op: string) (arg: Expr)
-  | EShiftAssign (op: string) (arg: Expr)
+  | EAssign (lval: nat) (arg: Expr)
+  | EShiftAssign (lval: nat) (arg: Expr)
   | ECond (cond tb fb: Expr)
   | EConcat (args: list Expr)
   | ERepl (amount: nat) (arg: Expr)
-  | EInside (arg: Expr) (range: list Expr)
+  | EInside (arg: Expr) (args: list Expr)
   .
 
   Set Elimination Schemes.
 
-  Section Expr_ind.
+  Section Expr_ind_gen.
     Variable P : Expr -> Prop.
     Variable P0 : list Expr -> Prop.
 
-    Hypothesis HPOperand:
-      forall o, P (EOperand o).
+    Hypothesis HPAtom:
+      forall o, P (EAtom o).
 
     Hypothesis HPBinOp:
       forall lhs rhs, P lhs -> P rhs -> P (EBinOp lhs rhs).
@@ -72,7 +74,7 @@ Module Expr.
       forall n arg, P arg -> P (ERepl n arg).
 
     Hypothesis HPInside:
-      forall arg range, P arg -> P0 range -> P (EInside arg range).
+      forall arg args, P arg -> P0 args -> P (EInside arg args).
 
     Hypothesis HP0Nil:
       P0 [].
@@ -80,31 +82,100 @@ Module Expr.
     Hypothesis HP0Cons:
       forall hd tl, P hd -> P0 tl -> P0 (hd :: tl).
 
-    Fixpoint Expr_ind e : P e.
+    Fixpoint Expr_ind_gen e : P e.
     Proof.
       destruct e.
-      - apply HPOperand.
-      - apply HPBinOp. apply Expr_ind. apply Expr_ind.
-      - apply HPUnOp. apply Expr_ind.
-      - apply HPCast. apply Expr_ind.
-      - apply HPComp. apply Expr_ind. apply Expr_ind.
-      - apply HPLogic. apply Expr_ind. apply Expr_ind.
-      - apply HPReduction. apply Expr_ind.
-      - apply HPShift. apply Expr_ind. apply Expr_ind.
-      - apply HPAssign. apply Expr_ind.
-      - apply HPShiftAssign. apply Expr_ind.
-      - apply HPCond. apply Expr_ind. apply Expr_ind. apply Expr_ind.
+      - apply HPAtom.
+      - apply HPBinOp. firstorder. firstorder.
+      - apply HPUnOp. firstorder.
+      - apply HPCast. firstorder.
+      - apply HPComp. firstorder. firstorder.
+      - apply HPLogic. firstorder. firstorder.
+      - apply HPReduction. firstorder.
+      - apply HPShift. firstorder. firstorder.
+      - apply HPAssign. firstorder.
+      - apply HPShiftAssign. firstorder.
+      - apply HPCond. firstorder. firstorder. firstorder.
       - apply HPConcat. induction args.
         + apply HP0Nil.
-        + apply HP0Cons. apply Expr_ind. apply IHargs.
-      - apply HPRepl. apply Expr_ind.
-      - apply HPInside. apply Expr_ind. induction range.
+        + apply HP0Cons. firstorder. firstorder.
+      - apply HPRepl. firstorder.
+      - apply HPInside. firstorder. induction args.
         + apply HP0Nil.
-        + apply HP0Cons. apply Expr_ind. apply IHrange.
-     Qed.
+        + apply HP0Cons. firstorder. firstorder.
+    Qed.
+  End Expr_ind_gen.
 
+  Section Expr_ind.
+    Variable P : Expr -> Prop.
+
+    Hypothesis HPAtom:
+      forall o, P (EAtom o).
+
+    Hypothesis HPBinOp:
+      forall lhs rhs, P lhs -> P rhs -> P (EBinOp lhs rhs).
+
+    Hypothesis HPUnOp:
+      forall arg, P arg -> P (EUnOp arg).
+
+    Hypothesis HPCast:
+      forall arg, P arg -> P (ECast arg).
+
+    Hypothesis HPComp:
+      forall lhs rhs, P lhs -> P rhs -> P (EComp lhs rhs).
+
+    Hypothesis HPLogic:
+      forall lhs rhs, P lhs -> P rhs -> P (ELogic lhs rhs).
+
+    Hypothesis HPReduction:
+      forall arg, P arg -> P (EReduction arg).
+
+    Hypothesis HPShift:
+      forall lhs rhs, P lhs -> P rhs -> P (EShift lhs rhs).
+
+    Hypothesis HPAssign:
+      forall op arg, P arg -> P (EAssign op arg).
+
+    Hypothesis HPShiftAssign:
+      forall op arg, P arg -> P (EShiftAssign op arg).
+
+    Hypothesis HPCond:
+      forall cond tb fb, P cond -> P tb -> P fb -> P (ECond cond tb fb).
+
+    Hypothesis HPConcat:
+      forall args, (forall n e, nth_error args n = Some e -> P e) -> P (EConcat args).
+
+    Hypothesis HPRepl:
+      forall n arg, P arg -> P (ERepl n arg).
+
+    Hypothesis HPInside:
+      forall arg args, P arg -> (forall n e, nth_error args n = Some e -> P e) ->
+                  P (EInside arg args).
+
+    Definition Expr_ind e : P e.
+    Proof.
+      induction e using Expr_ind_gen with
+        (P0 := fun args => forall n e, nth_error args n = Some e -> P e).
+      - firstorder.
+      - firstorder.
+      - firstorder.
+      - firstorder.
+      - firstorder.
+      - firstorder.
+      - firstorder.
+      - firstorder.
+      - firstorder.
+      - firstorder.
+      - firstorder.
+      - firstorder.
+      - firstorder.
+      - firstorder.
+      - intros. destruct n; discriminate H.
+      - intros. destruct n.
+        + inv H. apply IHe.
+        + apply (IHe0 _ _ H).
+    Qed.
    End Expr_ind.
-
 End Expr.
 
 
@@ -114,14 +185,11 @@ Module Notation.
   Declare Custom Entry expr.
   Declare Custom Entry expr_var.
 
-  Notation "a" := (ident_to_string! a) (in custom expr_var at level 0, a constr at level 0, only parsing).
-  Notation "a" := (a) (in custom expr_var at level 0, a constr at level 0, format " a ", only printing).
-
   Notation "$( x )" := x (in custom expr at level 0, x constr, only parsing).
-  Notation "<{ e }>" := e (e custom expr at level 200, only parsing).
+  Notation "<{ e }>" := e (e custom expr at level 200).
 
   Notation "( x )" := x (in custom expr at level 0, x custom expr).
-  Notation "x" := (EOperand x) (in custom expr at level 0, x custom expr_var at level 0).
+  Notation "x" := (EAtom x) (in custom expr at level 0, x constr at level 0).
   Notation "x + y" := (EBinOp x y) (in custom expr at level 50, left associativity).
   Notation "- x" := (EUnOp x) (in custom expr at level 0).
   Notation "'signed' ( x )" := (ECast x) (in custom expr at level 0).
