Rocq/src/Attempts/TwoWay.v
@@ -1,0 +1,112 @@
+From Stdlib Require Import Strings.String.
+From Stdlib Require Import Lists.List.
+From Stdlib Require Import PeanoNat.
+From Verilog Require Import Expr.
+From Verilog Require Import Path.
+From Verilog Require Import Utils.
+
+Import ListNotations.
+Import Nat.
+Import Expr.
+Import Path.
+Import Utils.
+
+Import Notation.
+
+Set Implicit Arguments.
+
+Module TwoWay.
+
+  Fixpoint sum (l: list nat) :=
+    match l with
+    | [] => 0
+    | hd :: tl => hd + sum tl
+    end
+  .
+
+  Fixpoint inside_max (s: nat) (l: list nat) :=
+    match l with
+    | [] => s
+    | hd :: tl => max hd (inside_max s tl)
+    end
+  .
+
+  Inductive type : nat -> Expr -> nat -> Prop :=
+  | TAtom : forall n s,
+      type n (EAtom s) s
+  | TBinOp : forall n a b s sa sb,
+      type n a sa -> type n b sb -> s = max sa sb -> type n (EBinOp a b) s
+  | TUnOp : forall n e s,
+      type n e s -> type n (EUnOp e) s
+  | TCast : forall n e s,
+      type s e s -> type n (ECast e) s
+  | TComp : forall n a b s sa sb,
+      type s a sa -> type s b sb -> s = max sa sb -> type n (EComp a b) 1
+  | TLogic : forall n a b sa sb,
+      type sa a sa -> type sb b sb -> type n (ELogic a b) 1
+  | TReduction : forall n e s,
+      type s e s -> type n (EReduction e) 1
+  | TShift : forall n a b s sb,
+      type n a s -> type sb b sb -> type n (EShift a b) s
+  | TAssign : forall n lval e ne se,
+      type ne e se -> ne = max se lval -> type n (EAssign lval e) lval
+  | TShiftAssign : forall n lval e se,
+      type se e se -> type n (EShiftAssign lval e) lval
+  | TCond : forall n e a b s se sa sb,
+      type se e se -> type n a se -> type n b sb -> s = max sa sb -> type n (ECond e a b) s
+  | TConcat : forall n args sargs s,
+      type_concat args sargs -> s = sum sargs -> type n (EConcat args) s
+  | TRepl : forall n amount e se s ,
+      type se e se -> s = se * amount -> type n (ERepl amount e) s
+  | TInside : forall n e args se sargs s,
+      type s e se -> type_inside s args sargs -> s = inside_max s sargs -> type n (EInside e args) 1
+
+  with type_concat : list Expr -> list nat -> Prop :=
+  | TConcatNil : type_concat [] []
+  | TConcatCons : forall e el s sl,
+      type s e s -> type_concat el sl -> type_concat (e :: el) (s :: sl)
+
+  with type_inside : nat -> list Expr -> list nat -> Prop :=
+  | TInsideNil : forall n, type_inside n [] []
+  | TInsideCons : forall n e el s sl,
+      type n e s -> type_inside n el sl -> type_inside n (e :: el) (s :: sl)
+  .
+
+  Scheme type_rec := Induction for type Sort Prop
+      with type_concat_rec := Induction for type_concat Sort Prop
+      with type_inside_rec := Induction for type_inside Sort Prop.
+
+  Definition ExprHasType e n := type n e n.
+
+  Definition e := <{ 10 + 2 + &(34) }>.
+
+  Lemma eType: forall n, n = 10 <-> ExprHasType e n.
+  Proof.
+    split; intros; subst.
+    - unfold e.
+      apply TBinOp with (sa := 10) (sb := 1).
+      + apply TBinOp with (sa := 10) (sb := 2).
+        * constructor.
+        * constructor.
+        * reflexivity.
+      + apply TReduction with (s := 34). constructor.
+      + reflexivity.
+    - inv H. inv H4. inv H2. inv H5. inv H3. reflexivity.
+  Qed.
+
+
+  Lemma concat: forall eList nList n,
+      length eList = length nList ->
+      ExprHasType (EConcat eList) n <->
+        (forall i f s, nth_error eList i = Some f
+                  -> nth_error nList i = Some s
+                  -> ExprHasType f s) /\ (n = sum nList).
+  Proof.
+    split; intros.
+    - split; intros.
+      + inv H0. generalize dependent nList. induction eList; intros.
+        * destruct i; discriminate H1.
+        * destruct i.
+          -- simpl in *. inv H1. destruct nList. discriminate H. inv H2. clear H.
+  Admitted.
+End TwoWay.
