Rocq/src/BiDir.v
@@ -1,0 +1,247 @@
+From Stdlib Require Import Strings.String.
+From Stdlib Require Import Lists.List.
+From Stdlib Require Import PeanoNat.
+From Verilog Require Import Expr.
+From Verilog Require Import Path.
+From Verilog Require Import Utils.
+
+Import ListNotations.
+Import Nat.
+Import Expr.
+Import Path.
+Import Utils.
+
+Set Implicit Arguments.
+
+Module BiDir.
+
+  Inductive Resizable : Expr -> Prop :=
+  | ResAtom : forall op, Resizable (EAtom op)
+  | ResCast : forall e, Resizable (ECast e)
+  | ResComp : forall lhs rhs, Resizable (EComp lhs rhs)
+  | ResLogic : forall lhs rhs, Resizable (ELogic lhs rhs)
+  | ResRed : forall e, Resizable (EReduction e)
+  | ResAssign : forall lval arg, Resizable (EAssign lval arg)
+  | ResShiftAssign : forall lval arg, Resizable (EShiftAssign lval arg)
+  | ResConcat : forall args, Resizable (EConcat args)
+  | ResRepl : forall amount arg, Resizable (ERepl amount arg)
+  | ResInside : forall arg args, Resizable (EInside arg args)
+  .
+
+  Fixpoint sum (l: list nat) :=
+    match l with
+    | [] => 0
+    | hd :: tl => hd + sum tl
+    end
+  .
+
+  Reserved Notation "e '==>' t" (at level 90).
+  Reserved Notation "e '==>l' t" (at level 90).
+  Reserved Notation "e '<==' t" (at level 90).
+  Reserved Notation "e '<==l' t" (at level 90).
+
+  Inductive synth : Expr -> nat -> Prop :=
+  | AtomS op : EAtom op ==> op
+
+  | LBinOpS a b t :
+      a ==> t ->
+      b <== t ->
+      (* ========== *)
+      EBinOp a b ==> t
+
+  | RBinOpS a b t :
+      a <== t ->
+      b ==> t ->
+      (* ========== *)
+      EBinOp a b ==> t
+
+  | UnOpS e t :
+    e ==> t ->
+    (* ========== *)
+    EUnOp e ==> t
+
+  | CastS e t :
+    e ==> t ->
+    (* ========== *)
+    ECast e ==> t
+
+  | LCompS a b t :
+    a ==> t ->
+    b <== t ->
+    (* ========== *)
+    EComp a b ==> 1
+
+  | RCompS a b t :
+    a <== t ->
+    b ==> t ->
+    (* ========== *)
+    EComp a b ==> 1
+
+  | LogicS a b ta tb :
+    a ==> ta ->
+    b ==> tb ->
+    (* ========== *)
+    ELogic a b ==> 1
+
+  | RedS e t :
+    e ==> t ->
+    (* ========== *)
+    EReduction e ==> 1
+
+  | Shift a b t tb :
+    a ==> t ->
+    b ==> tb ->
+    (* ========== *)
+    EShift a b ==> t
+
+  | LAssignS lval e :
+    e <== lval ->
+    (* ========== *)
+    EAssign lval e ==> lval
+
+  | RAssignS lval e te :
+    e ==> te ->
+    lval < te ->
+    (* ========== *)
+    EAssign lval e ==> lval
+
+  | AssignShiftS lval e te :
+    e ==> te ->
+    (* ========== *)
+    EShiftAssign lval e ==> lval
+
+  | LCondS e a b t te :
+    e ==> te ->
+    a ==> t ->
+    b <== t ->
+    (* ========== *)
+    ECond e a b ==> t
+
+  | RCondS e a b t te :
+    e ==> te ->
+    a <== t ->
+    b ==> t ->
+    (* ========== *)
+    ECond e a b ==> t
+
+  | ConcatS args ts t :
+    args ==>l ts ->
+    t = sum ts ->
+    (* ========== *)
+    EConcat args ==> t
+
+  | ReplS i e te t :
+    e ==> te ->
+    t = i * te ->
+    (* ========== *)
+    ERepl i e ==> t
+
+  | LInsideS a args t :
+    a ==> t ->
+    args <==l t ->
+    (* ========== *)
+    EInside a args ==> t
+
+  | RInsideS a args e t :
+    In e args ->
+    e ==> t ->
+    a <== t ->
+    args <==l t ->
+    (* ========== *)
+    EInside a args ==> t
+
+  where "e '==>' n" := (synth e n)
+
+  with synthList : list Expr -> list nat -> Prop :=
+  | SynthNil : [] ==>l []
+
+  | SynthCons e t eL tL :
+    e ==> t ->
+    eL ==>l tL ->
+    (* ========== *)
+    (e :: eL) ==>l (t :: tL)
+
+  where "e '==>l' n" := (synthList e n)
+
+  with check : Expr -> nat -> Prop :=
+  | ResizeC e s t :
+      Resizable e ->
+      e ==> s ->
+      s <= t ->
+      (* ========== *)
+      e <== t
+
+  | BinOpC a b t :
+      a <== t ->
+      b <== t ->
+      (* ========== *)
+      EBinOp a b <== t
+
+  | UnOpC e t :
+      e <== t ->
+      (* ========== *)
+      EUnOp e <== t
+
+  | ShiftC a b t tb :
+      a <== t ->
+      b ==> tb ->
+      (* ========== *)
+      EShift a b <== t
+
+  | CondC e a b t te :
+      e ==> te ->
+      a <== t ->
+      b <== t ->
+      (* ========== *)
+      ECond e a b <== t
+
+  where "e '<==' n" := (check e n)
+
+  with checkList : list Expr -> nat -> Prop :=
+  | CheckNil t : [] <==l t
+
+  | CheckCons e eL t :
+    e <== t ->
+    eL <==l t ->
+    (* ========== *)
+    (e :: eL) <==l t
+
+  where "e '<==l' n" := (checkList e n)
+  .
+
+
+  Lemma check_can_grow : forall e t s, e <== t -> t <= s -> e <== s.
+  Proof.
+    Ltac _check_can_grow_tac :=
+      match goal with
+      | [ HRes: Resizable _, H: ?e ==> ?x, Hle: ?x <= ?y |- ?e <== ?z ] =>
+          apply (ResizeC HRes H); apply (le_trans x y z); assumption
+      | [ H: _ <== _ |- _ <== _ ] => inv H; _check_can_grow_tac
+      end
+    .
+    induction e using Expr_ind; intros; try _check_can_grow_tac.
+    - inv H. inv H1. constructor. firstorder. firstorder.
+    - inv H. inv H1. constructor. firstorder.
+    - inv H. inv H1. assert (H : e1 <== s). firstorder. apply (ShiftC H H5).
+    - inv H. inv H1. apply (CondC H4). firstorder. firstorder.
+  Qed.
+
+  Theorem synth_can_check : forall e t, e ==> t -> forall s, t <= s -> e <== s.
+  Proof.
+    induction e using Expr_ind; intros;
+      try (apply ResizeC with (s := t0); [constructor | assumption | assumption]).
+    - inv H.
+      + constructor. firstorder. apply (check_can_grow H5 H0).
+      + constructor. apply (check_can_grow H3 H0). firstorder.
+    - inv H. constructor. firstorder.
+    - inv H. assert (H: e1 <== s). firstorder. apply (ShiftC H H5).
+    - inv H.
+      + apply (CondC H4). firstorder. apply (check_can_grow H7 H0).
+      + apply (CondC H4). apply (check_can_grow H6 H0). firstorder.
+  Qed.
+
+  Lemma synth_implies_check: forall e t, e ==> t -> e <== t.
+  Proof.
+    intros. apply synth_can_check with (t := t0). assumption. constructor.
+  Qed.
+End BiDir.
