Prolog/p.pl
@@ -1,0 +1,76 @@
+max(A, A, B) :- A >= B.
+max(B, A, B) :- B > A.
+
+lSize(S, S).
+atomSize(S, S).
+
+type_(_, atom(X), S) :-
+    atomSize(X, S).
+
+type_(N, binOp(A, B), S) :-
+    type_(N, A, Sa),
+    type_(N, B, Sb),
+    max(S, Sa, Sb).
+
+type_(N, unOp(E), S) :-
+    type_(N, E, S).
+
+type_(_, cast(E), S) :-
+    type_(S, E, S).
+
+type_(_, comp(A, B), 1) :-
+    type_(S, A, Sa),
+    type_(S, B, Sb),
+    max(S, Sa, Sb).
+
+type_(_, logic(A, B), 1) :-
+    type_(Sa, A, Sa),
+    type_(Sb, B, Sb).
+
+type_(_, red(E), 1) :-
+    type_(S, E, S).
+
+type_(N, shif(A, B), S) :-
+    type_(N, A, S),
+    type_(Sb, B, Sb).
+
+type_(_, assign(L, E), S) :-
+    lSize(L, S),
+    type_(Ne, E, Se),
+    max(Ne, S, Se).
+
+type_(_, shiftAssign(L, E), S) :-
+    lSize(L, S),
+    type_(Se, E, Se).
+
+type_(N, cond(E, A, B), S) :-
+    type_(Se, E, Se),
+    type_(N, A, Sa),
+    type_(N, B, Sb),
+    max(S, Sa, Sb).
+
+type_(_, concat(A, B), S) :-
+    type_(Sa, A, Sa),
+    type_(Sb, B, Sb),
+    S is Sa + Sb.
+
+type_(_, repl(I, E), S) :-
+    type_(Se, E, Se),
+    S is I * Se.
+
+show_type_(P, E, N) :-
+    nl,
+    write(P),
+    print(E),
+    write(': '),
+    print(N).
+
+% type_(N, E, S) :-
+%     show_type_('?  ', E, N),
+%     type_(N, E, S),
+%     show_type_('-> ', E, N).
+
+type(E, N) :- type_(N, E, N).
+
+% trace.
+% type_(cond(atom(4), binOp(red(atom(5)), cast(binOp(atom(1), atom(2)))), atom(32)), X).
